Revert to old option in Core/Framework

SSA/Core/Framework.lean
@@ -522,23 +522,24 @@ end Lemmas
 ## `denote`
 Denote expressions, programs, and sequences of lets
 -/
+variable [TyDenote d.Ty] [DialectDenote d] [DecidableEq d.Ty] [Monad d.m] [LawfulMonad d.m]
 
 mutual
 
-def HVector.denote [TyDenote d.Ty] [Monad d.m] [DialectDenote d] :
+def HVector.denote :
     {l : List (Ctxt d.Ty × d.Ty)} → (T : HVector (fun t => Com d t.1 .impure t.2) l) →
     HVector (fun t => t.1.Valuation → EffectKind.impure.toMonad d.m (toType t.2)) l
   | _, .nil => HVector.nil
   | _, .cons v vs => HVector.cons (v.denote) (HVector.denote vs)
 
-def Expr.denote [TyDenote d.Ty] [Monad d.m] [DialectDenote d] {ty : d.Ty} (e : Expr d Γ eff ty) (Γv : Valuation Γ) :
+def Expr.denote {ty : d.Ty} (e : Expr d Γ eff ty) (Γv : Valuation Γ) :
     eff.toMonad d.m (toType ty) :=
   match e with
   | ⟨op, Eq.refl _, heff, args, regArgs⟩ =>
     EffectKind.liftEffect heff <| DialectDenote.denote op
       (args.map (fun _ v => Γv v)) regArgs.denote
 
-def Com.denote [TyDenote d.Ty] [Monad d.m] [DialectDenote d] : Com d Γ eff ty → (Γv : Valuation Γ) → eff.toMonad d.m (toType ty)
+def Com.denote : Com d Γ eff ty → (Γv : Valuation Γ) → eff.toMonad d.m (toType ty)
   | .ret e, Γv => pure (Γv e)
   | .var e body, Γv =>
      match eff with
@@ -548,7 +549,7 @@ end
 
 /-- Denote just the let bindings of `com`, transforming a valuation for `Γ` into a valuation for
 the output context of `com` -/
-def Com.denoteLets [TyDenote d.Ty] [Monad d.m] [DialectDenote d] : (com : Com d Γ eff ty) → (Γv : Valuation Γ) →
+def Com.denoteLets : (com : Com d Γ eff ty) → (Γv : Valuation Γ) →
     eff.toMonad d.m (com.outContext.Valuation)
   | .ret _, V => pure V
   | .var e body, V =>
@@ -559,18 +560,18 @@ def Com.denoteLets [TyDenote d.Ty] [Monad d.m] [DialectDenote d] : (com : Com d 
 --TODO: this should be an abbrev: the `liftM` is inserted automatically when writing `e.denote`
 --      inside of `do`-notation, and we shouldn't have two ways to write the same thing
 /-- Denote an `Expr` in an unconditionally impure fashion -/
-def Expr.denoteImpure [TyDenote d.Ty] [Monad d.m] [DialectDenote d] (e : Expr d Γ eff ty) (Γv : Valuation Γ) :
+def Expr.denoteImpure (e : Expr d Γ eff ty) (Γv : Valuation Γ) :
     EffectKind.impure.toMonad d.m (toType ty) :=
   liftM <| e.denote Γv
 
 --TODO: figure out if we can write this in terms of `liftM`, too
 /-- Denote a `Com` in an unconditionally impure fashion -/
-def Com.denoteImpure [TyDenote d.Ty] [Monad d.m] [DialectDenote d] :
+def Com.denoteImpure :
     Com d Γ eff ty → (Γv : Valuation Γ) → EffectKind.impure.toMonad d.m (toType ty)
   | .ret e, Γv => pure (Γv e)
   | .var e body, Γv => e.denoteImpure Γv >>= fun x => body.denote (Γv.snoc x)
 
-def Lets.denote [TyDenote d.Ty] [Monad d.m] [DialectSignature d] [DialectDenote d] {Γ₂}
+def Lets.denote [DialectSignature d] [DialectDenote d] {Γ₂}
     (lets : Lets d Γ₁ eff Γ₂) (Γ₁'v : Valuation Γ₁) : (eff.toMonad d.m <| Valuation Γ₂) :=
   match lets with
   | .nil => return Γ₁'v
@@ -587,12 +588,12 @@ realize that `pure.toMonad d.m (Valuation _)` is just `Valuation _`, and thus a 
 Therefore, if a goalstate is `⊢ lets.denote ... = lets.denote ...`, and `lets` is pure, then to use
 the congruence, you can do: `rw [← Lets.denotePure]; congr`
 -/
-@[simp] abbrev Lets.denotePure [TyDenote d.Ty] [Monad d.m] [DialectSignature d] [DialectDenote d] :
+@[simp] abbrev Lets.denotePure [DialectSignature d] [DialectDenote d] :
     Lets d Γ₁ .pure Γ₂ → Valuation Γ₁ → Valuation Γ₂ := Lets.denote
 
 --TODO: figure out if we can write this in terms of `liftM`, too
 /-- Denote a `Lets` in an unconditionally impure fashion -/
-def Lets.denoteImpure [TyDenote d.Ty] [Monad d.m] [DialectSignature d] [DialectDenote d] {Γ₂}
+def Lets.denoteImpure [DialectSignature d] [DialectDenote d] {Γ₂}
     (lets : Lets d Γ₁ eff Γ₂) (Γ₁'v : Valuation Γ₁) :
     (EffectKind.impure.toMonad d.m <| Valuation Γ₂) :=
   match lets with
@@ -604,7 +605,7 @@ def Lets.denoteImpure [TyDenote d.Ty] [Monad d.m] [DialectSignature d] [DialectD
 
 /-- The denotation of a zipper is a composition of the denotations of the constituent
 `Lets` and `Com` -/
-def Zipper.denote [TyDenote d.Ty] [Monad d.m] [DialectDenote d] (zip : Zipper d Γ_in eff Γ_out ty) (V_in : Valuation Γ_in) :
+def Zipper.denote (zip : Zipper d Γ_in eff Γ_out ty) (V_in : Valuation Γ_in) :
     eff.toMonad d.m ⟦ty⟧ :=
   (zip.top.denote V_in) >>= zip.bot.denote
 
@@ -615,9 +616,6 @@ open EffectKind (liftEffect)
 /- Equation lemma to unfold `denote`, which does not unfold correctly due to the presence
   of the coercion `ty_eq` and the mutual definition. -/
 theorem Expr.denote_unfold
-    [TyDenote d.Ty]
-    [Monad d.m]
-    [DialectDenote d]
     (op : d.Op)
     (ty_eq : ty = DialectSignature.outTy op)
     (eff_le : DialectSignature.effectKind op ≤ eff)
@@ -633,7 +631,7 @@ theorem Expr.denote_unfold
 
 /-- Equation lemma to unfold `denote`, which does not unfold correctly due to the presence
   of the coercion `ty_eq` and the mutual definition. -/
-theorem Com.denote_unfold [TyDenote d.Ty] [Monad d.m] [DialectDenote d] (op : d.Op) (ty_eq : ty = DialectSignature.outTy op)
+theorem Com.denote_unfold (op : d.Op) (ty_eq : ty = DialectSignature.outTy op)
     (eff_le : DialectSignature.effectKind op ≤ eff)
     (args : HVector (Var Γ) <| DialectSignature.sig op)
     (regArgs : HVector (fun (t : Ctxt d.Ty × d.Ty) => Com d t.1 .impure t.2)
@@ -676,52 +674,46 @@ end Unfoldings
 section Lemmas
 
 @[simp] lemma HVector.denote_nil
-    [TyDenote d.Ty]
-    [Monad d.m]
-    [DialectDenote d]
     (T : HVector (fun (t : Ctxt d.Ty × d.Ty) => Com d t.1 .impure t.2) []) :
     HVector.denote T = HVector.nil := by
   cases T; simp [HVector.denote]
 
 @[simp] lemma HVector.denote_cons
-    [TyDenote d.Ty]
-    [Monad d.m]
-    [DialectDenote d]
     (t : Ctxt d.Ty × d.Ty) (ts : List (Ctxt d.Ty × d.Ty))
     (a : Com d t.1 .impure t.2) (as : HVector (fun t => Com d t.1 .impure t.2) ts) :
     HVector.denote (.cons a as) = .cons (a.denote) (as.denote) := by
   simp [HVector.denote]
 
-@[simp] lemma Com.denote_ret [TyDenote d.Ty] [Monad d.m] [DialectDenote d] {eff : EffectKind} (Γ : Ctxt d.Ty) (x : Γ.Var t) :
+@[simp] lemma Com.denote_ret {eff : EffectKind} (Γ : Ctxt d.Ty) (x : Γ.Var t) :
     (Com.ret x : Com d Γ eff t).denote = fun Γv => return (Γv x) := by
   funext Γv
   simp [denote]
 
-@[simp] lemma Com.denote_var [TyDenote d.Ty] [Monad d.m] [DialectDenote d] [LawfulMonad d.m] {e : Expr d Γ eff α} :
+@[simp] lemma Com.denote_var [LawfulMonad d.m] {e : Expr d Γ eff α} :
     (Com.var e body).denote =
     fun Γv => (e.denote Γv) >>= (fun v => body.denote (Γv.snoc v)) := by
   funext Γv
   cases eff <;> simp [denote]
 
-@[simp] lemma Com.denoteLets_var [TyDenote d.Ty] [Monad d.m] [DialectDenote d] (e : Expr d Γ eff t) (body : Com d _ eff u) [LawfulMonad d.m] :
+@[simp] lemma Com.denoteLets_var (e : Expr d Γ eff t) (body : Com d _ eff u) [LawfulMonad d.m] :
     (Com.var e body).denoteLets =
         (fun V => e.denote V >>= fun Ve => body.denoteLets (V.snoc Ve)) := by
   funext V
   cases eff <;> simp [denoteLets, bind_pure]
 
-@[simp] lemma Com.denoteImpure_ret [TyDenote d.Ty] [Monad d.m] [DialectDenote d] {Γ : Ctxt d.Ty} (x : Γ.Var t) :
+@[simp] lemma Com.denoteImpure_ret [Monad d.m] [DialectDenote d] {Γ : Ctxt d.Ty} (x : Γ.Var t) :
   (Com.ret (d:=d) (eff := eff) x).denoteImpure = fun Γv => return (Γv x) := rfl
 
-@[simp] lemma Com.denoteImpure_body [TyDenote d.Ty] [Monad d.m] [DialectDenote d] {Γ : Ctxt d.Ty}
+@[simp] lemma Com.denoteImpure_body [Monad d.m] [DialectDenote d] {Γ : Ctxt d.Ty}
     (e : Expr d Γ eff te) (body : Com d (Γ.snoc te) eff tbody) :
   (Com.var e body).denoteImpure =
   fun Γv => e.denoteImpure Γv >>= fun x => body.denote (Γv.snoc x) := rfl
 
-@[simp] lemma Lets.denote_nil [TyDenote d.Ty] [Monad d.m] [DialectDenote d] {Γ : Ctxt d.Ty} :
+@[simp] lemma Lets.denote_nil {Γ : Ctxt d.Ty} :
     (Lets.nil : Lets d Γ eff Γ).denote = (return ·) := by
   funext; simp [denote]
 
-@[simp] lemma Lets.denote_var [TyDenote d.Ty] [Monad d.m] [DialectDenote d] {lets : Lets d Γ_in eff Γ_out} {e : Expr d Γ_out eff t} :
+@[simp] lemma Lets.denote_var {lets : Lets d Γ_in eff Γ_out} {e : Expr d Γ_out eff t} :
     (lets.var e).denote = fun V_in => (do
       let V_out ← lets.denote V_in
       let x ← e.denote V_out
@@ -731,10 +723,6 @@ section Lemmas
 
 
 @[simp] lemma Lets.denote_addComToEnd
-    [TyDenote d.Ty]
-    [Monad d.m]
-    [DialectDenote d]
-    [LawfulMonad d.m]
     {lets : Lets d Γ_in eff Γ_out} {com : Com d Γ_out eff t} :
     Lets.denote (lets.addComToEnd com) = fun V => (do
         let Vlets ← lets.denote V
@@ -745,10 +733,10 @@ section Lemmas
   case ret => simp [Lets.denote_var, Com.denoteLets]
   case var ih => simp [addComToEnd, ih, denote_var]
 
-@[simp] lemma Com.denoteLets_ret [TyDenote d.Ty] [Monad d.m] [DialectDenote d] : (.ret v : Com d Γ eff t).denoteLets = fun V => pure V := by
+@[simp] lemma Com.denoteLets_ret : (.ret v : Com d Γ eff t).denoteLets = fun V => pure V := by
   funext V; simp [denoteLets]
 
-theorem Com.denoteLets_eq [TyDenote d.Ty] [Monad d.m] [DialectDenote d] [LawfulMonad d.m] {com : Com d Γ eff t} : com.denoteLets = com.toLets.denote := by
+theorem Com.denoteLets_eq {com : Com d Γ eff t} : com.denoteLets = com.toLets.denote := by
   simp only [toLets]; induction com using Com.rec' <;> simp [Lets.denote_var]
 
 end Lemmas
@@ -773,7 +761,7 @@ def Com.changeVars : Com d Γ eff ty →
 
 /-! simp-lemmas about `changeVars`-/
 
-@[simp] lemma Expr.denote_changeVars [TyDenote d.Ty] [Monad d.m] [DialectDenote d] {Γ Γ' : Ctxt d.Ty}
+@[simp] lemma Expr.denote_changeVars {Γ Γ' : Ctxt d.Ty}
     (varsMap : Γ.Hom Γ')
     (e : Expr d Γ eff ty) :
     (e.changeVars varsMap).denote =
@@ -797,9 +785,6 @@ def Com.changeVars : Com d Γ eff ty →
   ((Com.ret (d:=d) (eff := eff) v).changeVars varsMap).outContext = Γ' := by simp
 
 @[simp] lemma Com.denote_changeVars
-    [TyDenote d.Ty]
-    [Monad d.m]
-    [DialectDenote d]
     (varsMap : Γ.Hom Γ') (c : Com d Γ eff ty) :
     (c.changeVars varsMap).denote =
     c.denote ∘ (fun V => V.comap varsMap) := by
@@ -812,7 +797,7 @@ def Com.changeVars : Com d Γ eff ty →
     simp only [changeVars_var]
     split <;> simp_all
 
-@[simp] lemma Com.denote_changeVars' [TyDenote d.Ty] [Monad d.m] [DialectDenote d] (varsMap : Γ.Hom Γ') (c : Com d Γ eff ty) :
+@[simp] lemma Com.denote_changeVars' (varsMap : Γ.Hom Γ') (c : Com d Γ eff ty) :
     (c.changeVars varsMap).denote = fun V => c.denote (V.comap varsMap) := by
   simp; rfl
 
@@ -822,7 +807,7 @@ def Com.changeVars : Com d Γ eff ty →
   | .var _ body  => cast (by simp) <|
       Com.outContext_changeVars_hom (map := map.snocMap) map_inv.snocMap (c := body)
 
-@[simp] lemma Com.denoteLets_returnVar_pure [TyDenote d.Ty] [Monad d.m] [DialectDenote d] (c : Com d Γ .pure ty) (Γv : Valuation Γ) :
+@[simp] lemma Com.denoteLets_returnVar_pure (c : Com d Γ .pure ty) (Γv : Valuation Γ) :
     c.denoteLets Γv c.returnVar = c.denote Γv := by
   induction c using Com.recPure <;> simp_all [denoteLets, denote]
 
@@ -846,21 +831,21 @@ structure FlatCom (d : Dialect) [DialectSignature d]  (Γ_in : Ctxt d.Ty) (eff :
 
 --TODO: should this be a `@[simp] abbrev`, or just nuked altogether?
 /-- Denote the Lets of the FlatICom -/
-def FlatCom.denoteLets [TyDenote d.Ty] [Monad d.m] [DialectDenote d] (flatCom : FlatCom d Γ eff Γ_out t) (Γv : Γ.Valuation) :
+def FlatCom.denoteLets (flatCom : FlatCom d Γ eff Γ_out t) (Γv : Γ.Valuation) :
     eff.toMonad d.m <| Γ_out.Valuation :=
   flatCom.lets.denote Γv
 
 /-- Denote the lets and the ret of the FlatCom. This is equal to denoting the Com -/
-@[simp] abbrev FlatCom.denote [TyDenote d.Ty] [Monad d.m] [DialectDenote d] (flatCom : FlatCom d Γ eff Γ_out t)
+@[simp] abbrev FlatCom.denote [DialectDenote d] (flatCom : FlatCom d Γ eff Γ_out t)
     (Γv : Γ.Valuation) : eff.toMonad d.m (toType t) :=
   flatCom.lets.denote Γv >>= fun Γ'v => return (Γ'v flatCom.ret)
 
-theorem FlatCom.denoteLets_eq [TyDenote d.Ty] [Monad d.m] [DialectDenote d] (flatCom : FlatCom d Γ eff Γ_out t) :
+theorem FlatCom.denoteLets_eq [DialectDenote d] (flatCom : FlatCom d Γ eff Γ_out t) :
     flatCom.denoteLets = fun Γv => flatCom.lets.denote Γv := by
   funext Γv
   simp [denoteLets]
 
-theorem FlatCom.denote_eq [TyDenote d.Ty] [Monad d.m] [DialectDenote d] (flatCom : FlatCom d Γ eff Γ_out t) :
+theorem FlatCom.denote_eq [DialectDenote d] (flatCom : FlatCom d Γ eff Γ_out t) :
     flatCom.denote = fun Γv => flatCom.lets.denote Γv >>= fun Γ'v => return (Γ'v flatCom.ret) := by
   funext Γv
   simp [denote]
@@ -969,7 +954,7 @@ section Lemmas
 
 /-! denotations of `castPureToEff` -/
 
-@[simp] lemma Expr.denote_castPureToEff [TyDenote d.Ty] [Monad d.m] [DialectDenote d] {e : Expr d Γ .pure t} :
+@[simp] lemma Expr.denote_castPureToEff {e : Expr d Γ .pure t} :
     denote (e.castPureToEff eff) = fun V => pure (e.denote V) := by
   rcases e with ⟨op, rfl, eff_le, _, _⟩
   cases eff
@@ -980,12 +965,12 @@ section Lemmas
       EffectKind.liftEffect_pure,
       EffectKind.liftEffect_eq_pure_cast (EffectKind.eq_of_le_pure eff_le)]
 
-@[simp] lemma Com.denote_castPureToEff [TyDenote d.Ty] [Monad d.m] [DialectDenote d] [LawfulMonad d.m] {com : Com d Γ .pure ty} :
+@[simp] lemma Com.denote_castPureToEff {com : Com d Γ .pure ty} :
     denote (com.castPureToEff eff) = fun V => pure (com.denote V) := by
   funext V; simp only [EffectKind.return_impure_toMonad_eq]
   induction com using Com.recPure <;> simp_all
 
-@[simp] lemma Com.denoteLets_castPureToEff [TyDenote d.Ty] [Monad d.m] [DialectDenote d] [LawfulMonad d.m] {com : Com d Γ .pure ty} :
+@[simp] lemma Com.denoteLets_castPureToEff {com : Com d Γ .pure ty} :
     denoteLets (com.castPureToEff eff)
     = fun V => pure (com.denoteLets V |>.comap fun _ v => v.castCtxt (by simp)) := by
   funext V; induction com using Com.recPure <;> simp_all
@@ -1017,7 +1002,7 @@ theorem Expr.HasPureOp_of_pure : (e : Expr d Γ .pure t) → e.HasPureOp
   | ⟨_, _, eff_le, _, _⟩ => EffectKind.eq_of_le_pure eff_le
 
 /-- Rewrite theorem for an expression with a pure operation (which might be evaluated impurely) -/
-theorem Expr.denote_mk_of_pure [TyDenote d.Ty] [Monad d.m] [DialectDenote d] {op : d.Op} (eff_eq : DialectSignature.effectKind op = .pure)
+theorem Expr.denote_mk_of_pure {op : d.Op} (eff_eq : DialectSignature.effectKind op = .pure)
     (ty_eq : ty = _) (eff_le : DialectSignature.effectKind op ≤ eff₂)
     (args : HVector (Var Γ) (DialectSignature.sig op))
     (regArgs : HVector (fun (t : Ctxt d.Ty × d.Ty) => Com d t.1 EffectKind.impure t.2)
@@ -1046,7 +1031,7 @@ theorem Expr.denote_mk_of_pure [TyDenote d.Ty] [Monad d.m] [DialectDenote d] {op
     · simp
     · symm; simp
 
-theorem Expr.denote_of_pure [TyDenote d.Ty] [Monad d.m] [DialectDenote d] {e : Expr d Γ eff ty} (eff_eq : e.HasPureOp) :
+theorem Expr.denote_of_pure {e : Expr d Γ eff ty} (eff_eq : e.HasPureOp) :
     e.denote = (fun (Γv : Valuation Γ) =>
       let d : EffectKind.toMonad .pure d.m ⟦ty⟧ :=
         cast (by rw [eff_eq, ← e.ty_eq]) <|
@@ -1063,7 +1048,7 @@ theorem Expr.denote_of_pure [TyDenote d.Ty] [Monad d.m] [DialectDenote d] {e : E
 /-- casting an expr to an impure expr and running it equals running it purely
 and returning the value -/
 @[simp]
-theorem Expr.denote_castPureToEff_impure_eq [TyDenote d.Ty] [Monad d.m] [DialectDenote d] [LawfulMonad d.m] (e : Expr d Γ .pure t) :
+theorem Expr.denote_castPureToEff_impure_eq [LawfulMonad d.m] (e : Expr d Γ .pure t) :
     (e.castPureToEff .impure).denote = fun Γv => return (e.denote Γv) := by
   rcases e with ⟨op, ty_eq, eff_le, args, regArgs⟩
   simp only [castPureToEff, changeEffect, denote_mk_of_pure (EffectKind.eq_of_le_pure eff_le)]
@@ -1082,7 +1067,7 @@ theorem Expr.hasPureOp_of_toPure?_isSome {e : Expr d Γ eff ty} (h : e.toPure?.i
     next => contradiction
 
 /-- The denotation of toPure? -/
-theorem Expr.denote_toPure? [TyDenote d.Ty] [Monad d.m] [DialectDenote d] {e : Expr d Γ eff ty} {e': Expr d Γ .pure ty}
+theorem Expr.denote_toPure? {e : Expr d Γ eff ty} {e': Expr d Γ .pure ty}
     (he : Expr.toPure? e = some e') : e.denote =
     match eff with
     | .pure => e'.denote
@@ -1127,7 +1112,7 @@ def Zipper.toCom (zip : Zipper d Γ_in eff Γ_mid ty) : Com d Γ_in eff ty :=
 
 /-- Add a `Com` directly before the current position of a zipper, while reassigning every
 occurence of a given free variable (`v`) of `zip.com` to the output of the new `Com`  -/
-def Zipper.insertCom [DecidableEq d.Ty] (zip : Zipper d Γ_in eff Γ_mid ty) (v : Var Γ_mid newTy)
+def Zipper.insertCom (zip : Zipper d Γ_in eff Γ_mid ty) (v : Var Γ_mid newTy)
     (newCom : Com d Γ_mid eff newTy) : Zipper d Γ_in eff newCom.outContext ty :=
   let newTop := zip.top.addComToEnd newCom
   --  ^^^^^^ The combination of the previous `top` with the `newCom` inserted
@@ -1142,7 +1127,7 @@ zipper, while r eassigning every occurence of a given free variable (`v`) of
 
 This is a wrapper around `insertCom` (which expects `newCom` to have the same effect as `zip`)
 and `castPureToEff` -/
-def Zipper.insertPureCom [DecidableEq d.Ty] (zip : Zipper d Γ_in eff Γ_mid ty) (v : Var Γ_mid newTy)
+def Zipper.insertPureCom (zip : Zipper d Γ_in eff Γ_mid ty) (v : Var Γ_mid newTy)
     (newCom : Com d Γ_mid .pure newTy) : Zipper d Γ_in eff newCom.outContext ty :=
   (by simp : (newCom.castPureToEff eff).outContext = newCom.outContext)
     ▸ zip.insertCom v (newCom.castPureToEff eff)
@@ -1154,15 +1139,15 @@ section Lemmas
 @[simp] lemma Zipper.toCom_var {lets : Lets d Γ_in eff Γ_mid} :
     Zipper.toCom ⟨Lets.var lets e, com⟩ = Zipper.toCom ⟨lets, Com.var e com⟩ := rfl
 
-@[simp] theorem Zipper.denote_toCom [TyDenote d.Ty] [Monad d.m] [DialectDenote d] [LawfulMonad d.m] (zip : Zipper d Γ_in eff Γ_mid ty) :
+@[simp] theorem Zipper.denote_toCom [LawfulMonad d.m] (zip : Zipper d Γ_in eff Γ_mid ty) :
     zip.toCom.denote = zip.denote := by
   rcases zip with ⟨lets, com⟩
   funext Γv; induction lets <;> simp [Lets.denote, Zipper.denote, *]
 
-@[simp] lemma Zipper.denote_mk [TyDenote d.Ty] [Monad d.m] [DialectDenote d] {lets : Lets d Γ_in eff Γ_out} {com : Com d Γ_out eff ty} :
+@[simp] lemma Zipper.denote_mk {lets : Lets d Γ_in eff Γ_out} {com : Com d Γ_out eff ty} :
     denote ⟨lets, com⟩ = fun V => (lets.denote V) >>= com.denote := rfl
 
-theorem Zipper.denote_insertCom [TyDenote d.Ty] [Monad d.m] [DialectDenote d] [DecidableEq d.Ty] {zip : Zipper d Γ_in eff Γ_mid ty₁}
+theorem Zipper.denote_insertCom {zip : Zipper d Γ_in eff Γ_mid ty₁}
     {newCom : Com d _ eff newTy} [LawfulMonad d.m] :
     (zip.insertCom v newCom).denote = (fun (V_in : Valuation Γ_in) => do
       let V_mid ← zip.top.denote V_in
@@ -1174,12 +1159,12 @@ theorem Zipper.denote_insertCom [TyDenote d.Ty] [Monad d.m] [DialectDenote d] [D
   simp [insertCom, Com.denoteLets_eq, Function.comp]
 
 /-- Casting the intermediate context is not relevant for the denotation -/
-@[simp] lemma Zipper.denoteLets_eqRec_Γ_mid [TyDenote d.Ty] [Monad d.m] [DialectDenote d] {zip : Zipper d Γ_in eff Γ_mid ty}
+@[simp] lemma Zipper.denoteLets_eqRec_Γ_mid {zip : Zipper d Γ_in eff Γ_mid ty}
     (h : Γ_mid = Γ_mid') :
     denote (h ▸ zip) = zip.denote := by
   subst h; rfl
 
-theorem Zipper.denote_insertPureCom [TyDenote d.Ty] [Monad d.m] [DialectDenote d] [DecidableEq d.Ty] {zip : Zipper d Γ_in eff Γ_mid ty₁}
+theorem Zipper.denote_insertPureCom {zip : Zipper d Γ_in eff Γ_mid ty₁}
     {newCom : Com d _ .pure newTy} [LawfulMonad d.m] :
     (zip.insertPureCom v newCom).denote = (fun (V_in : Valuation Γ_in) => do
       let V_mid ← zip.top.denote V_in
@@ -1213,14 +1198,14 @@ section DenoteInsert
 
 /-- Denoting any of the free variables of a program through `Com.denoteLets` just returns the
 assignment of that variable in the input valuation -/
-@[simp] lemma Com.denoteLets_outContextHom [TyDenote d.Ty] [Monad d.m] [DialectDenote d] (com : Com d Γ .pure ty) (V : Valuation Γ)
+@[simp] lemma Com.denoteLets_outContextHom (com : Com d Γ .pure ty) (V : Valuation Γ)
     {vTy} (v : Var Γ vTy) :
     com.denoteLets V (com.outContextHom v) = V v := by
   induction com using Com.recPure
   · simp
   · rw [outContextHom_var]; simp [denoteLets, *]
 
-@[simp] lemma Ctxt.Valuation.comap_outContextHom_denoteLets [TyDenote d.Ty] [Monad d.m] [DialectDenote d] {com : Com d Γ .pure ty} {V} :
+@[simp] lemma Ctxt.Valuation.comap_outContextHom_denoteLets {com : Com d Γ .pure ty} {V} :
     Valuation.comap (com.denoteLets V) com.outContextHom = V := by
   unfold comap; simp
 
@@ -1296,7 +1281,7 @@ def Lets.getPureExpr {Γ₁ Γ₂ : Ctxt d.Ty} (lets : Lets d Γ₁ eff Γ₂) {
     Expr.changeVars_changeVars];
   rfl
 
-theorem Lets.denote_getPureExprAux [TyDenote d.Ty] [Monad d.m] [DialectDenote d] [LawfulMonad d.m] {Γ₁ Γ₂ : Ctxt d.Ty} {t : d.Ty}
+theorem Lets.denote_getPureExprAux [LawfulMonad d.m] {Γ₁ Γ₂ : Ctxt d.Ty} {t : d.Ty}
     {lets : Lets d Γ₁ eff Γ₂} {v : Var Γ₂ t} {ePure : Expr d _ .pure t}
     (he : lets.getPureExprAux v = some ePure)
     (s : Valuation Γ₁)
@@ -1330,7 +1315,7 @@ theorem Lets.denote_getPureExprAux [TyDenote d.Ty] [Monad d.m] [DialectDenote d]
         Valuation.snoc_last]
       cases eff <;> simp
 
-theorem Lets.denote_getExpr [TyDenote d.Ty] [Monad d.m] [DialectDenote d] [LawfulMonad d.m] {Γ₁ Γ₂ : Ctxt d.Ty}
+theorem Lets.denote_getExpr [LawfulMonad d.m] {Γ₁ Γ₂ : Ctxt d.Ty}
     {lets : Lets d Γ₁ eff Γ₂} {t : d.Ty}
     {v : Var Γ₂ t} {e : Expr d Γ₂ .pure t} (he : lets.getPureExpr v = some e) (s : Valuation Γ₁) :
     (f : Valuation Γ₂ → ⟦t⟧ → eff.toMonad d.m α) →
@@ -1495,18 +1480,18 @@ end AListTheorems
 -/
 
 /-- Convert a heterogenous vector of variables into a homogeneous `VarSet` -/
-def HVector.toVarSet [DecidableEq d.Ty] : {l : List d.Ty} → (T : HVector (Var Γ) l) → VarSet Γ
+def HVector.toVarSet : {l : List d.Ty} → (T : HVector (Var Γ) l) → VarSet Γ
   | [], .nil => ∅
   | _::_, .cons v vs => insert ⟨_, v⟩ vs.toVarSet
 
 -- TODO: `HVector.toVarSet` and `HVector.vars` do the same thing, deduplicate
-def HVector.vars [DecidableEq d.Ty] {l : List d.Ty} (T : HVector (Var Γ) l) : VarSet Γ :=
+def HVector.vars {l : List d.Ty} (T : HVector (Var Γ) l) : VarSet Γ :=
   T.foldl (fun _ s a => insert ⟨_, a⟩ s) ∅
 
 --TODO: find a name that better encapsulates that it's the *transitive* closure
 /-- The free variables of `lets` that are (transitively) referred to by some variable `v`.
 Also known as the uses of var. -/
-def Lets.vars [DecidableEq d.Ty] : Lets d Γ_in eff Γ_out → Var Γ_out t → VarSet Γ_in
+def Lets.vars : Lets d Γ_in eff Γ_out → Var Γ_out t → VarSet Γ_in
   | .nil, v => VarSet.ofVar v
   | .var lets e, v => by
       cases v using Var.casesOn with
@@ -1516,20 +1501,21 @@ def Lets.vars [DecidableEq d.Ty] : Lets d Γ_in eff Γ_out → Var Γ_out t → 
 
 /-- `com.vars` is the set of free variables from `Γ` that are (transitively) used by the return
 variable of `com` -/
-def Com.vars [DecidableEq d.Ty] : Com d Γ .pure t → VarSet Γ :=
+def Com.vars : Com d Γ .pure t → VarSet Γ :=
   fun com => com.toFlatCom.lets.vars com.toFlatCom.ret
 
-theorem Lets.vars_var_eq [DecidableEq d.Ty] {lets : Lets d Γ_in eff Γ_out}
+theorem Lets.vars_var_eq {lets : Lets d Γ_in eff Γ_out}
   {t: d.Ty} {e : Expr d Γ_out eff t}
   {w : ℕ} {tw : d.Ty} {wh : Ctxt.get? Γ_out w = some tw} :
   Lets.vars (Lets.var lets e) ⟨w + 1, by simpa [Ctxt.snoc] using wh⟩ =
   Lets.vars lets ⟨w, wh⟩ := by simp [Lets.vars]
 
-@[simp] lemma HVector.vars_nil [DecidableEq d.Ty] :
-  (HVector.nil : HVector (Var Γ) ([] : List d.Ty)).vars = ∅ := by
-simp [HVector.vars, HVector.foldl]
 
-@[simp] lemma HVector.vars_cons [DecidableEq d.Ty] {t  : d.Ty} {l : List d.Ty}
+@[simp] lemma HVector.vars_nil :
+    (HVector.nil : HVector (Var Γ) ([] : List d.Ty)).vars = ∅ := by
+  simp [HVector.vars, HVector.foldl]
+
+@[simp] lemma HVector.vars_cons {t  : d.Ty} {l : List d.Ty}
     (v : Var Γ t) (T : HVector (Var Γ) l) :
     (HVector.cons v T).vars = insert ⟨_, v⟩ T.vars := by
   rw [HVector.vars, HVector.vars]
@@ -1549,7 +1535,7 @@ simp [HVector.vars, HVector.foldl]
   let s₁ and s₂ be two maps from variables to A t.
   If s₁ and s₂ agree on all variables in T (which is a VarSet),
   then T.map s₁ = T.map s₂ -/
-theorem HVector.map_eq_of_eq_on_vars [DecidableEq d.Ty] {A : d.Ty → Type*}
+theorem HVector.map_eq_of_eq_on_vars {A : d.Ty → Type*}
     {T : HVector (Var Γ) l}
     {s₁ s₂ : ∀ (t), Var Γ t → A t}
     (h : ∀ v, v ∈ T.vars → s₁ _ v.2 = s₂ _ v.2) :
@@ -1651,7 +1637,7 @@ instance : DialectSignature (TermModel d Γ) where
 instance : TyDenote (TermModel d Γ).Ty where
   toType := fun ty => ExprTree d Γ ty.1
 
-instance [Monad d.m] [p : PureDialect d] : DialectDenote (TermModel d Γ) where
+instance [p : PureDialect d] : DialectDenote (TermModel d Γ) where
   denote := fun op args _regArgs =>
     return .mk op rfl (p.allPure _) (argsToBranches args)
   where
@@ -1684,7 +1670,7 @@ variable [PureDialect d]
 
 /-- `lets.toSubstitution` gives a substitution from each variable in the output context to an
 expression tree with variables in the input context by following the def-use chain -/
-def Lets.toSubstitution [Monad d.m] (lets : Lets d Γ_in .pure Γ_out) : Γ_out.Substitution d Γ_in :=
+def Lets.toSubstitution (lets : Lets d Γ_in .pure Γ_out) : Γ_out.Substitution d Γ_in :=
   Ctxt.Substitution.ofValuation <|
     (lets.changeDialect TermModel.morphism).denote fun ⟨ty⟩ ⟨v, h⟩ =>
       ExprTree.fvar ⟨v, by
@@ -1723,7 +1709,7 @@ mutual
 /-- `matchArg lets matchLets args matchArgs map` tries to extends the partial substition `map` by
 calling `matchVar lets args[i] matchLets matchArgs[i]` for each pair of corresponding variables,
 returning the final partial substiution, or `none` on conflicting assigments -/
-def matchArg [DecidableEq d.Ty] [DecidableEq d.Op]
+def matchArg [DecidableEq d.Op]
     (lets : Lets d Γ_in eff Γ_out) (matchLets : Lets d Δ_in .pure Δ_out) :
     {l : List d.Ty} → HVector (Var Γ_out) l → HVector (Var Δ_out) l →
     Mapping Δ_in Γ_out → Option (Mapping Δ_in Γ_out)
@@ -1750,7 +1736,7 @@ This obeys the hypothetical equation: `(matchLets.exprTreeAt w).changeVars map =
 where `exprTreeAt` is a hypothetical definition that gives the expression tree.
 
 NOTE: this only matches on *pure* let bindings in both `matchLets` and `lets`. -/
-def matchVar [DecidableEq d.Ty] {Γ_in Γ_out Δ_in Δ_out : Ctxt d.Ty} {t : d.Ty} [DecidableEq d.Op]
+def matchVar {Γ_in Γ_out Δ_in Δ_out : Ctxt d.Ty} {t : d.Ty} [DecidableEq d.Op]
     (lets : Lets d Γ_in eff Γ_out) (v : Var Γ_out t) :
     (matchLets : Lets d Δ_in .pure Δ_out) →
     (w : Var Δ_out t) →
@@ -1798,7 +1784,7 @@ def matchVar [DecidableEq d.Ty] {Γ_in Γ_out Δ_in Δ_out : Ctxt d.Ty} {t : d.T
 end
 
 /-- how matchVar behaves on `var` at a successor variable -/
-theorem matchVar_var_succ_eq [DecidableEq d.Ty] {Γ_in Γ_out Δ_in Δ_out : Ctxt d.Ty} {t te : d.Ty} [DecidableEq d.Op]
+theorem matchVar_var_succ_eq {Γ_in Γ_out Δ_in Δ_out : Ctxt d.Ty} {t te : d.Ty} [DecidableEq d.Op]
     (lets : Lets d Γ_in eff Γ_out) (v : Var Γ_out t)
     (matchLets : Lets d Δ_in .pure Δ_out)
     (matchE : Expr d Δ_out .pure te)
@@ -1814,7 +1800,7 @@ theorem matchVar_var_succ_eq [DecidableEq d.Ty] {Γ_in Γ_out Δ_in Δ_out : Ctx
       unfold matchVar
 
 /-- how matchVar behaves on `var` at the last variable. -/
-theorem matchVar_var_last_eq [DecidableEq d.Ty] {Γ_in Γ_out Δ_in Δ_out : Ctxt d.Ty} {t : d.Ty} [DecidableEq d.Op]
+theorem matchVar_var_last_eq {Γ_in Γ_out Δ_in Δ_out : Ctxt d.Ty} {t : d.Ty} [DecidableEq d.Op]
     (lets : Lets d Γ_in eff Γ_out) (v : Var Γ_out t)
     (matchLets : Lets d Δ_in .pure Δ_out)
     (matchE : Expr d Δ_out .pure t)
@@ -1832,10 +1818,9 @@ theorem matchVar_var_last_eq [DecidableEq d.Ty] {Γ_in Γ_out Δ_in Δ_out : Ctx
 
 section SubsetEntries
 
-theorem subset_entries [TyDenote d.Ty] [Monad d.m] :
+theorem subset_entries :
     (
-     ∀  (Γ_in : Ctxt d.Ty) (eff : EffectKind) (Γ_out Δ_in Δ_out : Ctxt d.Ty)
-        (inst' : DecidableEq d.Ty)
+     ∀ (Γ_in : Ctxt d.Ty) (eff : EffectKind) (Γ_out Δ_in Δ_out : Ctxt d.Ty)
         (inst : DecidableEq d.Op)
         (lets : Lets d Γ_in eff Γ_out)
         (matchLets : Lets d Δ_in EffectKind.pure Δ_out) (l : List d.Ty)
@@ -1843,10 +1828,7 @@ theorem subset_entries [TyDenote d.Ty] [Monad d.m] :
       ∀ varMap ∈ matchArg lets matchLets argsl argsr ma, ma.entries ⊆ varMap.entries
     )
     ∧ (
-      ∀ (eff : EffectKind)
-        (inst' : DecidableEq d.Ty)
-        (Γ_in Γ_out Δ_in Δ_out : Ctxt d.Ty) (t : d.Ty)
-        (inst : DecidableEq d.Op)
+      ∀ (eff : EffectKind) (Γ_in Γ_out Δ_in Δ_out : Ctxt d.Ty) (t : d.Ty) (inst : DecidableEq d.Op)
         (lets : Lets d Γ_in eff Γ_out) (v : Γ_out.Var t)
         (matchLets : Lets d Δ_in EffectKind.pure Δ_out)
         (w : Var Δ_out t) (ma : Mapping Δ_in Γ_out),
@@ -1855,13 +1837,13 @@ theorem subset_entries [TyDenote d.Ty] [Monad d.m] :
   apply matchArg.mutual_induct (d:=d)
   <;> first
       | intro (Γ_in : Ctxt _) eff Γ_out Δ_in Δ_out inst lets matchLets
-      | intro (eff : EffectKind) _ Γ_in Γ_out  Δ_in t inst lets w
-  · intro _ ma varMap hvarMap
+      | intro (eff : EffectKind) Γ_in Γ_out Δ_in t inst lets w
+  · intro ma varMap hvarMap
     simp [matchArg, Option.mem_def, Option.some.injEq] at hvarMap
     subst hvarMap
     exact Set.Subset.refl _
 
-  · intro _ t inst vl argsl matchLets argsr ma ih_matchVar ih_matchArg varMap hvarMap
+  · intro t inst vl argsl matchLets argsr ma ih_matchVar ih_matchArg varMap hvarMap
     simp only [matchArg, bind, Option.mem_def, Option.bind_eq_some] at hvarMap
     rcases hvarMap with ⟨ma', h1, h2⟩
     have hind : ma'.entries ⊆ _ := ih_matchArg ma' varMap <| by
@@ -1929,7 +1911,7 @@ theorem subset_entries [TyDenote d.Ty] [Monad d.m] :
       · subst hx; simp_all
       · rwa [AList.lookup_insert_ne hx]
 
-theorem subset_entries_matchArg [TyDenote d.Ty] [Monad d.m] [DecidableEq d.Ty] [DecidableEq d.Op]
+theorem subset_entries_matchArg [DecidableEq d.Op]
     {Γ_out Δ_in Δ_out : Ctxt d.Ty}
     {lets : Lets d Γ_in eff Γ_out}
     {matchLets : Lets d Δ_in .pure Δ_out}
@@ -1940,7 +1922,7 @@ theorem subset_entries_matchArg [TyDenote d.Ty] [Monad d.m] [DecidableEq d.Ty] [
     {varMap : Mapping Δ_in Γ_out}
     (hvarMap : varMap ∈ matchArg lets matchLets argsl argsr ma) :
     ma.entries ⊆ varMap.entries :=
-  subset_entries.1 _ _ _ _ _ _ _ _ _ _ _ _ _ _  hvarMap
+  subset_entries.1 _ _ _ _ _ _ _ _ _ _ _ _ _ hvarMap
 
 /--
 matchVar only adds new entries:
@@ -1948,26 +1930,22 @@ matchVar only adds new entries:
   then ma is a subset of varMap.
 Said differently, The output mapping of `matchVar` extends the input mapping when it succeeds.
 -/
-theorem subset_entries_matchVar [TyDenote d.Ty] [Monad d.m] [DecidableEq d.Ty] [DecidableEq d.Op]
+theorem subset_entries_matchVar [DecidableEq d.Op]
     {varMap : Mapping Δ_in Γ_out} {ma : Mapping Δ_in Γ_out}
     {lets : Lets d Γ_in eff Γ_out} {v : Var Γ_out t}
     {matchLets : Lets d Δ_in .pure Δ_out}
     {w : Var Δ_out t}
     (hvarMap : varMap ∈ matchVar lets v matchLets w ma) :
     ma.entries ⊆ varMap.entries :=
-  subset_entries.2 _ _ _ _ _ _ _ _ _ _ _ _ _ _ hvarMap
+  subset_entries.2 _ _ _ _ _ _ _ _ _ _ _ _ _ hvarMap
 
 end SubsetEntries
 
+
 -- TODO: this assumption is too strong, we also want to be able to model non-inhabited types
-variable [TyDenote d.Ty] in
 variable [∀ (t : d.Ty), Inhabited (toType t)] [DecidableEq d.Op]
 
 theorem denote_matchVar_matchArg
-    [TyDenote d.Ty]
-    [Monad d.m]
-    [DecidableEq d.Op]
-    [DecidableEq d.Ty]
     {Γ_out Δ_in Δ_out : Ctxt d.Ty} {lets : Lets d Γ_in eff Γ_out}
     {matchLets : Lets d Δ_in .pure Δ_out} :
     {l : List d.Ty} →
@@ -1998,6 +1976,8 @@ theorem denote_matchVar_matchArg
     · exact h_sub
     · exact hmatchVar
 
+variable [LawfulMonad d.m]
+
 section DenoteIntoSubtype
 
 /- TODO: we might not need `denoteIntoSubtype`, if we can prove that `V ∈ supp (lets.denote _)`
@@ -2006,10 +1986,10 @@ implies `lets.getPureExpr v = some e → e.denote V = V v` -/
 /-- `e.IsDenotationForPureE Γv x` holds if `x` is the pure value obtained from `e` under valuation
 `Γv`, assuming that `e` has a pure operation.
 If `e` has an impure operation, the property holds vacuously. -/
-abbrev Expr.IsDenotationForPureE [TyDenote d.Ty] [Monad d.m] [DialectDenote d] (e : Expr d Γ eff ty) (Γv : Valuation Γ) (x : ⟦ty⟧) : Prop :=
+abbrev Expr.IsDenotationForPureE (e : Expr d Γ eff ty) (Γv : Valuation Γ) (x : ⟦ty⟧) : Prop :=
   ∀ (ePure : Expr d Γ .pure ty), e.toPure? = some ePure → ePure.denote Γv = x
 
-def Expr.denoteIntoSubtype  [TyDenote d.Ty][Monad d.m] [DialectDenote d] (e : Expr d Γ_in eff ty) (Γv : Valuation Γ_in) :
+def Expr.denoteIntoSubtype (e : Expr d Γ_in eff ty) (Γv : Valuation Γ_in) :
     eff.toMonad d.m {x : ⟦ty⟧ // e.IsDenotationForPureE Γv x} :=
   match h_pure : e.toPure? with
     | some ePure => pure ⟨ePure.denote Γv, by simp [IsDenotationForPureE, h_pure]⟩
@@ -2020,7 +2000,7 @@ agrees with the denotation of every pure expression in `lets`.
 
 Strongly prefer using `Lets.denote` in definitions, but you can use `denoteIntoSubtype` in proofs.
 The subtype allows us to carry the property with us when doing congruence proofs inside a bind. -/
-def Lets.denoteIntoSubtype  [TyDenote d.Ty][Monad d.m] [DialectDenote d] (lets : Lets d Γ_in eff Γ_out) (Γv : Valuation Γ_in) :
+def Lets.denoteIntoSubtype (lets : Lets d Γ_in eff Γ_out) (Γv : Valuation Γ_in) :
     eff.toMonad d.m {
       V : Valuation Γ_out // ∀ {t} (v : Var _ t) e, lets.getPureExpr v = some e → e.denote V = V v
     } :=
@@ -2035,7 +2015,7 @@ def Lets.denoteIntoSubtype  [TyDenote d.Ty][Monad d.m] [DialectDenote d] (lets :
           · simpa using v.prop
           ⟩
 
-theorem Expr.denote_eq_denoteIntoSubtype [TyDenote d.Ty] [Monad d.m] [LawfulMonad d.m] [DialectDenote d] (e : Expr d Γ eff ty) (Γv : Valuation Γ) :
+theorem Expr.denote_eq_denoteIntoSubtype (e : Expr d Γ eff ty) (Γv : Valuation Γ) :
     e.denote Γv = Subtype.val <$> e.denoteIntoSubtype Γv := by
   simp only [denoteIntoSubtype, EffectKind.return_impure_toMonad_eq]
   split
@@ -2044,7 +2024,7 @@ theorem Expr.denote_eq_denoteIntoSubtype [TyDenote d.Ty] [Monad d.m] [LawfulMona
     split <;> rfl
   next => simp [map_eq_pure_bind]
 
-theorem Lets.denote_eq_denoteIntoSubtype [TyDenote d.Ty] [Monad d.m] [LawfulMonad d.m] [DialectDenote d] (lets : Lets d Γ_in eff Γ_out) (Γv : Valuation Γ_in) :
+theorem Lets.denote_eq_denoteIntoSubtype (lets : Lets d Γ_in eff Γ_out) (Γv : Valuation Γ_in) :
     lets.denote Γv = Subtype.val <$> (lets.denoteIntoSubtype Γv) := by
   induction lets
   case nil => simp [denoteIntoSubtype]
@@ -2054,7 +2034,7 @@ theorem Lets.denote_eq_denoteIntoSubtype [TyDenote d.Ty] [Monad d.m] [LawfulMona
 
 end DenoteIntoSubtype
 
-theorem matchVar_nil [DecidableEq d.Op] [DecidableEq d.Ty] {lets : Lets d Γ_in eff Γ_out} :
+theorem matchVar_nil {lets : Lets d Γ_in eff Γ_out} :
     matchVar lets v (.nil : Lets d Δ .pure Δ) w ma = some ma' →
     ma'.lookup ⟨_, w⟩ = some v := by
   unfold matchVar
@@ -2071,7 +2051,7 @@ theorem matchVar_nil [DecidableEq d.Op] [DecidableEq d.Ty] {lets : Lets d Γ_in 
     injection h with h
     simp [← h]
 
-theorem matchVar_var_last [DecidableEq d.Op] [DecidableEq d.Ty] {lets : Lets d Γ_in eff Γ_out} {matchLets : Lets d Δ_in .pure Δ_out}
+theorem matchVar_var_last {lets : Lets d Γ_in eff Γ_out} {matchLets : Lets d Δ_in .pure Δ_out}
     {matchExpr : Expr d Δ_out .pure ty} :
     matchVar lets v (.var matchLets matchExpr) (Var.last ..) ma = some ma' →
     ∃ args,
@@ -2089,12 +2069,12 @@ theorem matchVar_var_last [DecidableEq d.Op] [DecidableEq d.Ty] {lets : Lets d �
   subst regArgs_eq
   simpa using h
 
-@[simp] lemma Lets.denote_var_last_pure [TyDenote d.Ty] [Monad d.m] [DialectDenote d] (lets : Lets d Γ_in .pure Γ_out)
+@[simp] lemma Lets.denote_var_last_pure (lets : Lets d Γ_in .pure Γ_out)
     (e : Expr d Γ_out .pure ty) (V_in : Valuation Γ_in) :
     Lets.denote (var lets e) V_in (Var.last ..) = e.denote (lets.denote V_in) := by
   simp [Lets.denote]
 
-@[simp] lemma Expr.denote_eq_denote_of [TyDenote d.Ty] [Monad d.m] [DialectDenote d] {e₁ : Expr d Γ eff ty} {e₂ : Expr d Δ eff ty}
+@[simp] lemma Expr.denote_eq_denote_of {e₁ : Expr d Γ eff ty} {e₂ : Expr d Δ eff ty}
     {Γv : Valuation Γ} {Δv : Valuation Δ}
     (op_eq : e₁.op = e₂.op)
     (h_regArgs : HEq e₁.regArgs e₂.regArgs)
@@ -2108,8 +2088,7 @@ theorem matchVar_var_last [DecidableEq d.Op] [DecidableEq d.Ty] {lets : Lets d �
   subst ty_eq h_regArgs
   rw [denote, denote, h_args]
 
-variable [TyDenote d.Ty] [∀ (t : d.Ty), Inhabited (toType t)] [DecidableEq d.Op] in
-theorem denote_matchVar2_of_subset [Monad d.m] [LawfulMonad d.m] [DialectDenote d] [DecidableEq d.Ty]
+theorem denote_matchVar2_of_subset
     {lets : Lets d Γ_in eff Γ_out} {v : Var Γ_out t}
     {varMap₁ varMap₂ : Mapping Δ_in Γ_out}
     {s₁ : Valuation Γ_in}
@@ -2153,8 +2132,6 @@ theorem denote_matchVar2_of_subset [Monad d.m] [LawfulMonad d.m] [DialectDenote 
       · intro t v₁ v₂ ma ma' hmem h_ma_sub
         apply ih h_ma_sub hmem
       · exact (fun _ _ _ _ _ h => subset_entries_matchVar h)
-
-variable [TyDenote d.Ty] [∀ (t : d.Ty), Inhabited (toType t)] [DecidableEq d.Op] in
 /--
 if matchVar lets v matchLets w ma = .some varMap,
 then informally:
@@ -2162,7 +2139,7 @@ then informally:
    Γ_in --⟦lets⟧--> Γ_out --comap ma--> Δ_in --⟦matchLets⟧ --> Δ_out --w--> t =
      Γ_in ⟦lets⟧ --> Γ_out --v--> t
 -/
-theorem denote_matchVar2 [Monad d.m] [LawfulMonad d.m] [DialectDenote d] [DecidableEq d.Ty] {lets : Lets d Γ_in eff Γ_out} {v : Var Γ_out t}
+theorem denote_matchVar2 {lets : Lets d Γ_in eff Γ_out} {v : Var Γ_out t}
     {varMap : Mapping Δ_in Γ_out}
     {s₁ : Valuation Γ_in}
     {ma : Mapping Δ_in Γ_out}
@@ -2187,11 +2164,8 @@ macro_rules | `(tactic| decreasing_trivial) => `(tactic| simp (config := {arith 
 
 mutual
 
+
 theorem mem_matchVar_matchArg
-    [TyDenote d.Ty]
-    [Monad d.m] [LawfulMonad d.m]
-    [DecidableEq d.Op]
-    [DecidableEq d.Ty]
     {Γ_in Γ_out Δ_in Δ_out : Ctxt d.Ty}
     {lets : Lets d Γ_in eff Γ_out}
     {matchLets : Lets d Δ_in .pure Δ_out}
@@ -2201,7 +2175,7 @@ theorem mem_matchVar_matchArg
     (hvarMap : varMap ∈ matchArg lets matchLets argsₗ argsᵣ ma)
     {t' v'} : ⟨t', v'⟩ ∈ (argsᵣ.vars).biUnion (fun v => matchLets.vars v.2) → ⟨t', v'⟩ ∈ varMap :=
   match l, argsₗ, argsᵣ/- , ma, varMap, hvarMap -/ with
-  | .nil, .nil, .nil /- , _, varMap, _ -/ => by rw [HVector.vars_nil];simp only [Finset.biUnion_empty];simp only [Finset.not_mem_empty];simp only [false_implies]
+  | .nil, .nil, .nil /- , _, varMap, _ -/ => by simp
   | .cons t ts, .cons vₗ argsₗ, .cons vᵣ args /-, ma, varMap, h -/ => by
     simp only [matchArg, bind, Option.mem_def, Option.bind_eq_some] at hvarMap
     rcases hvarMap with ⟨ma', h₁, h₂⟩
@@ -2216,7 +2190,6 @@ theorem mem_matchVar_matchArg
 
 /-- All variables containing in `matchExpr` are assigned by `matchVar`. -/
 theorem mem_matchVar
-    [TyDenote d.Ty] [Monad d.m] [LawfulMonad d.m] [DecidableEq d.Ty] [DecidableEq d.Op]
     {varMap : Mapping Δ_in Γ_out} {ma : Mapping Δ_in Γ_out}
     {lets : Lets d Γ_in eff Γ_out} {v : Var Γ_out t} /- : -/
     {matchLets : Lets d Δ_in .pure Δ_out}  {w : Var Δ_out t}
@@ -2275,19 +2248,18 @@ theorem mem_matchVar
     subst h
     split_ifs at he₂ with h
     · dsimp only [Expr.op_mk, Expr.regArgs_mk] at h
-      apply mem_matchVar_matchArg (matchLets := matchLets) (hvarMap := he₂)
+      apply @mem_matchVar_matchArg (matchLets := matchLets) (hvarMap := he₂)
       simp only [Expr.op_mk, Finset.mem_biUnion, Sigma.exists]
       refine ⟨_, _, ?_, h_v'⟩
       rcases matchE  with ⟨_, _, _⟩
       dsimp only [Expr.op_mk, Expr.regArgs_mk] at h
       rcases h with ⟨rfl, _⟩
       exact hl
-
 end
 
 /-- A version of `matchVar` that returns a `Hom` of `Ctxt`s instead of the `AList`,
 provided every variable in the context appears as a free variable in `matchExpr`. -/
-def matchVarMap [TyDenote d.Ty] [DecidableEq d.Op] [Monad d.m] [LawfulMonad d.m] [DecidableEq d.Ty] {Γ_in Γ_out Δ_in Δ_out : Ctxt d.Ty} {t : d.Ty}
+def matchVarMap {Γ_in Γ_out Δ_in Δ_out : Ctxt d.Ty} {t : d.Ty}
     (lets : Lets d Γ_in eff Γ_out) (v : Var Γ_out t)
     (matchLets : Lets d Δ_in .pure Δ_out) (w : Var Δ_out t)
     (hvars : ∀ t (v : Var Δ_in t), ⟨t, v⟩ ∈ matchLets.vars w) :
@@ -2308,11 +2280,10 @@ def matchVarMap [TyDenote d.Ty] [DecidableEq d.Op] [Monad d.m] [LawfulMonad d.m]
             (hvarMap := by simp; apply hm) (hvars t v'))
       simp_all
 
-variable [TyDenote d.Ty] [∀ (t : d.Ty), Inhabited (toType t)] [DecidableEq d.Op] in
 /-- if matchVarMap lets v matchLets w hvars = .some map,
 then ⟦lets; matchLets⟧ = ⟦lets⟧(v)
 -/
-theorem denote_matchVarMap2 [DialectDenote d] [DecidableEq d.Ty] [Monad d.m] [LawfulMonad d.m] {Γ_in Γ_out Δ_in Δ_out : Ctxt d.Ty}
+theorem denote_matchVarMap2 [LawfulMonad d.m] {Γ_in Γ_out Δ_in Δ_out : Ctxt d.Ty}
     {lets : Lets d Γ_in eff Γ_out}
     {t : d.Ty} {v : Var Γ_out t}
     {matchLets : Lets d Δ_in .pure Δ_out}
@@ -2355,7 +2326,7 @@ def splitProgramAtAux : (pos : ℕ) → (lets : Lets d Γ₁ eff Γ₂) →
   | n+1, lets, .var e body =>
     splitProgramAtAux n (lets.var e) body
 
-theorem denote_splitProgramAtAux [TyDenote d.Ty] [DialectDenote d] [Monad d.m] [LawfulMonad d.m] : {pos : ℕ} → {lets : Lets d Γ₁ eff Γ₂} →
+theorem denote_splitProgramAtAux [LawfulMonad d.m] : {pos : ℕ} → {lets : Lets d Γ₁ eff Γ₂} →
     {prog : Com d Γ₂ eff t} →
     {res : Σ (Γ₃ : Ctxt d.Ty), Lets d Γ₁ eff Γ₃ × Com d Γ₃ eff t × (t' : d.Ty) × Var Γ₃ t'} →
     (hres : res ∈ splitProgramAtAux pos lets prog) →
@@ -2387,7 +2358,7 @@ def splitProgramAt (pos : ℕ) (prog : Com d Γ₁ eff t) :
     Option (Σ (Γ₂ : Ctxt d.Ty), Lets d Γ₁ eff Γ₂ × Com d Γ₂ eff t × (t' : d.Ty) × Var Γ₂ t') :=
   splitProgramAtAux pos .nil prog
 
-theorem denote_splitProgramAt [TyDenote d.Ty] [DialectDenote d] [Monad d.m] [LawfulMonad d.m] {pos : ℕ} {prog : Com d Γ₁ eff t}
+theorem denote_splitProgramAt [LawfulMonad d.m] {pos : ℕ} {prog : Com d Γ₁ eff t}
     {res : Σ (Γ₂ : Ctxt d.Ty), Lets d Γ₁ eff Γ₂ × Com d Γ₂ eff t × (t' : d.Ty) × Var Γ₂ t'}
     (hres : res ∈ splitProgramAt pos prog) (s : Valuation Γ₁) :
      (res.2.1.denote s) >>= res.2.2.1.denote = prog.denote s := by
@@ -2402,7 +2373,7 @@ theorem denote_splitProgramAt [TyDenote d.Ty] [DialectDenote d] [Monad d.m] [Law
 `target`. If it can match the variables, it inserts `rhs` into the program
 with the correct assignment of variables, and then replaces occurences
 of the variable at position `pos` in `target` with the output of `rhs`.  -/
-def rewriteAt [DecidableEq d.Op] [TyDenote d.Ty] [Monad d.m] [LawfulMonad d.m] [DecidableEq d.Ty] (lhs rhs : Com d Γ₁ .pure t₁)
+def rewriteAt (lhs rhs : Com d Γ₁ .pure t₁)
     (hlhs : ∀ t (v : Var Γ₁ t), ⟨t, v⟩ ∈ lhs.vars)
     (pos : ℕ) (target : Com d Γ₂ eff t₂) :
     Option (Com d Γ₂ eff t₂) := do
@@ -2417,16 +2388,15 @@ def rewriteAt [DecidableEq d.Op] [TyDenote d.Ty] [Monad d.m] [LawfulMonad d.m] [
     return zip.toCom
   else none
 
-@[simp] lemma Com.denote_toFlatCom_lets [TyDenote d.Ty] [Monad d.m] [DialectDenote d] [LawfulMonad d.m] (com : Com d Γ .pure t) :
+@[simp] lemma Com.denote_toFlatCom_lets [LawfulMonad d.m] (com : Com d Γ .pure t) :
     com.toFlatCom.lets.denote = com.denoteLets := by
   funext Γv; simp [toFlatCom, Com.denoteLets_eq]
 
-@[simp] lemma Com.toFlatCom_ret [Monad d.m] [LawfulMonad d.m] (com : Com d Γ .pure t) :
+@[simp] lemma Com.toFlatCom_ret [LawfulMonad d.m] (com : Com d Γ .pure t) :
     com.toFlatCom.ret = com.returnVar := by
   simp [toFlatCom]
 
-variable [TyDenote d.Ty] [∀ (t : d.Ty), Inhabited (toType t)] [DecidableEq d.Op] in
-theorem denote_rewriteAt [Monad d.m] [DecidableEq d.Ty] [DialectDenote d] [LawfulMonad d.m] (lhs rhs : Com d Γ₁ .pure t₁)
+theorem denote_rewriteAt [LawfulMonad d.m] (lhs rhs : Com d Γ₁ .pure t₁)
     (hlhs : ∀ t (v : Var Γ₁ t), ⟨t, v⟩ ∈ lhs.vars)
     (pos : ℕ) (target : Com d Γ₂ eff t₂)
     (hl : lhs.denote = rhs.denote)
@@ -2470,7 +2440,7 @@ structure PeepholeRewrite (Γ : List d.Ty) (t : d.Ty) where
   rhs : Com d (.ofList Γ) .pure t
   correct : lhs.denote = rhs.denote
 
-instance [DecidableEq d.Ty] {Γ : List d.Ty} {t' : d.Ty} {lhs : Com d (.ofList Γ) .pure t'} :
+instance {Γ : List d.Ty} {t' : d.Ty} {lhs : Com d (.ofList Γ) .pure t'} :
     Decidable (∀ (t : d.Ty) (v : Var (.ofList Γ) t), ⟨t, v⟩ ∈ lhs.vars) :=
   decidable_of_iff
     (∀ (i : Fin Γ.length),
@@ -2486,7 +2456,7 @@ instance [DecidableEq d.Ty] {Γ : List d.Ty} {t' : d.Ty} {lhs : Com d (.ofList �
   · intro h i
     apply h
 
-def rewritePeepholeAt [DecidableEq d.Op] [TyDenote d.Ty] [Monad d.m] [LawfulMonad d.m] [DecidableEq d.Ty] [DialectDenote d] (pr : PeepholeRewrite d Γ t)
+def rewritePeepholeAt (pr : PeepholeRewrite d Γ t)
     (pos : ℕ) (target : Com d Γ₂ eff t₂) :
     (Com d Γ₂ eff t₂) := if hlhs : ∀ t (v : Var (.ofList Γ) t), ⟨_, v⟩ ∈ pr.lhs.vars then
       match rewriteAt pr.lhs pr.rhs hlhs pos target
@@ -2495,8 +2465,8 @@ def rewritePeepholeAt [DecidableEq d.Op] [TyDenote d.Ty] [Monad d.m] [LawfulMona
         | none => target
       else target
 
-variable [TyDenote d.Ty] [∀ (t : d.Ty), Inhabited (toType t)] [DecidableEq d.Op] in
-theorem denote_rewritePeepholeAt [Monad d.m] [LawfulMonad d.m] [DecidableEq d.Ty] [DialectDenote d] (pr : PeepholeRewrite d Γ t)
+
+theorem denote_rewritePeepholeAt (pr : PeepholeRewrite d Γ t)
     (pos : ℕ) (target : Com d Γ₂  eff t₂) :
     (rewritePeepholeAt pr pos target).denote = target.denote := by
     simp only [rewritePeepholeAt]
@@ -2517,7 +2487,7 @@ section SimpPeepholeApplier
 
 /-- rewrite with `pr` to `target` program, at location `ix` and later, running
 at most `fuel` steps. -/
-def rewritePeephole_go [DecidableEq d.Op] [TyDenote d.Ty] [Monad d.m] [LawfulMonad d.m] [DecidableEq d.Ty] [DialectDenote d] (fuel : ℕ) (pr : PeepholeRewrite d Γ t)
+def rewritePeephole_go (fuel : ℕ) (pr : PeepholeRewrite d Γ t)
     (ix : ℕ) (target : Com d Γ₂ eff t₂) : (Com d Γ₂ eff t₂) :=
   match fuel with
   | 0 => target
@@ -2526,24 +2496,22 @@ def rewritePeephole_go [DecidableEq d.Op] [TyDenote d.Ty] [Monad d.m] [LawfulMon
      rewritePeephole_go fuel' pr (ix + 1) target'
 
 /-- rewrite with `pr` to `target` program, running at most `fuel` steps. -/
-def rewritePeephole [DecidableEq d.Op] [TyDenote d.Ty] [Monad d.m] [LawfulMonad d.m] [DecidableEq d.Ty] [DialectDenote d] (fuel : ℕ)
+def rewritePeephole (fuel : ℕ)
     (pr : PeepholeRewrite d Γ t) (target : Com d Γ₂ eff t₂) : (Com d Γ₂ eff t₂) :=
   rewritePeephole_go fuel pr 0 target
 
-variable [TyDenote d.Ty] [∀ (t : d.Ty), Inhabited (toType t)] [DecidableEq d.Op] in
 /-- `rewritePeephole_go` preserve semantics -/
-theorem denote_rewritePeephole_go [Monad d.m] [LawfulMonad d.m] [DecidableEq d.Ty] [DialectDenote d] (pr : PeepholeRewrite d Γ t)
+theorem denote_rewritePeephole_go (pr : PeepholeRewrite d Γ t)
     (pos : ℕ) (target : Com d Γ₂ eff t₂) :
     (rewritePeephole_go fuel pr pos target).denote = target.denote := by
   induction fuel generalizing pr pos target
   case zero =>
     simp[rewritePeephole_go, denote_rewritePeepholeAt]
   case succ fuel' hfuel =>
-    simp [rewritePeephole_go, hfuel, denote_rewritePeepholeAt]
+    simp[rewritePeephole_go, denote_rewritePeepholeAt, hfuel]
 
-variable [TyDenote d.Ty] [∀ (t : d.Ty), Inhabited (toType t)] [DecidableEq d.Op] in
 /-- `rewritePeephole` preserves semantics. -/
-theorem denote_rewritePeephole [Monad d.m] [LawfulMonad d.m] [DecidableEq d.Ty] [DialectDenote d] (fuel : ℕ)
+theorem denote_rewritePeephole (fuel : ℕ)
     (pr : PeepholeRewrite d Γ t) (target : Com d Γ₂ eff t₂) :
     (rewritePeephole fuel pr target).denote = target.denote := by
   simp[rewritePeephole, denote_rewritePeephole_go]
@@ -2551,7 +2519,7 @@ theorem denote_rewritePeephole [Monad d.m] [LawfulMonad d.m] [DecidableEq d.Ty] 
 /-- info: 'denote_rewritePeephole' depends on axioms: [propext, Classical.choice, Quot.sound] -/
 #guard_msgs in #print axioms denote_rewritePeephole
 
-theorem Expr.denote_eq_of_region_denote_eq [DecidableEq d.Op] [TyDenote d.Ty] [Monad d.m] [LawfulMonad d.m] [DecidableEq d.Ty] [DialectDenote d] (op : d.Op)
+theorem Expr.denote_eq_of_region_denote_eq (op : d.Op)
     (ty_eq : ty = DialectSignature.outTy op)
     (eff' : DialectSignature.effectKind op ≤ eff)
     (args : HVector (Var Γ) (DialectSignature.sig op))
@@ -2569,10 +2537,9 @@ theorem Expr.denote_eq_of_region_denote_eq [DecidableEq d.Op] [TyDenote d.Ty] [M
     subst ty_eq
     simp [Expr.denote, hregArgs']
 
-variable [TyDenote d.Ty] [∀ (t : d.Ty), Inhabited (toType t)] [DecidableEq d.Op] in
 mutual
 
-def rewritePeepholeRecursivelyRegArgs [Monad d.m] [LawfulMonad d.m] [DecidableEq d.Ty] [DialectDenote d] (fuel : ℕ)
+def rewritePeepholeRecursivelyRegArgs (fuel : ℕ)
     (pr : PeepholeRewrite d Γ t) {ts :  List (Ctxt d.Ty × d.Ty)}
     (args : HVector (fun t => Com d t.1 EffectKind.impure t.2) ts)
     : { out : HVector (fun t => Com d t.1 EffectKind.impure t.2) ts // out.denote = args.denote} :=
@@ -2587,7 +2554,7 @@ def rewritePeepholeRecursivelyRegArgs [Monad d.m] [LawfulMonad d.m] [DecidableEq
       let ⟨coms', hcoms'⟩ := (rewritePeepholeRecursivelyRegArgs fuel pr coms)
       ⟨.cons com' coms', by simp [hcom', hcoms']⟩
 
-def rewritePeepholeRecursivelyExpr [Monad d.m] [LawfulMonad d.m] [DecidableEq d.Ty] [DialectDenote d] (fuel : ℕ)
+def rewritePeepholeRecursivelyExpr (fuel : ℕ)
     (pr : PeepholeRewrite d Γ t) {ty : d.Ty}
     (e : Expr d Γ₂ eff ty) : { out : Expr d Γ₂ eff ty // out.denote = e.denote } :=
   match e with
@@ -2598,7 +2565,7 @@ def rewritePeepholeRecursivelyExpr [Monad d.m] [LawfulMonad d.m] [DecidableEq d.
 
 /-- A peephole rewriter that recurses into regions, allowing
 peephole rewriting into nested code. -/
-def rewritePeepholeRecursively [Monad d.m] [LawfulMonad d.m] [DecidableEq d.Ty] [DialectDenote d] (fuel : ℕ)
+def rewritePeepholeRecursively (fuel : ℕ)
     (pr : PeepholeRewrite d Γ t) (target : Com d Γ₂ eff t₂) :
     { out : Com d Γ₂ eff t₂ // out.denote = target.denote } :=
   match fuel with
